bump to v4.3.0-rc1, and make ReduceBool test deterministic

Lean4Checker/Tests/ReduceBool.lean
@@ -1,7 +1,22 @@
+open System IO.FS
+
+def t : FilePath := ".lean4checker.tmp"
+
+def exists_or_touch (f : FilePath) : IO Bool := do
+  match ← f.pathExists with
+  | false => writeFile f "0"; return true
+  | true => match ← readFile f with
+    | "0" => writeFile f "1"; return true
+    | "1" => writeFile f "2"; return true
+    | "2" => writeFile f "3"; return false
+    | "3" => writeFile f "4"; return false
+    | "4" => removeFile f; return false
+    | _ => throw <| IO.userError ""
+
 def foo : Bool :=
-  match IO.getRandomBytes 1 () with
-  | .ok bs _ => bs[0]! >= 128
+  match exists_or_touch t () with
+  | .ok b _ => b
   | _ => false
-theorem T1 : false = Lean.reduceBool foo := rfl
-theorem T2 : Lean.reduceBool foo = true := rfl
+theorem T1 : true = Lean.reduceBool foo := rfl
+theorem T2 : Lean.reduceBool foo = false := rfl
 theorem contradiction : False := nomatch T1.trans T2
